---
layout: post
title: "Thoughts on the Dihedral Hidden Subgroup Problem"
tags: maths cs
---

{% raw %}

  <p>This morning, I've been thinking again about a way to solve the <a href="http://en.wikipedia.org/wiki/Hidden_subgroup_problem">Hidden Subgroup Problem</a> for the <a href="http://en.wikipedia.org/wiki/Dihedral_group">dihedral group</a> <math xmlns="http://www.w3.org/1998/Math/MathML"> <msub> <mi>D</mi> <mi>N</mi> </msub> <mo>=</mo> <msub> <mi>ℤ</mi> <mi>N</mi> </msub> <msub> <mo>⋊</mo> <mi>φ</mi> </msub> <msub> <mi>ℤ</mi> <mn>2</mn> </msub> </math> (where <math xmlns="http://www.w3.org/1998/Math/MathML"> <mi>φ</mi> <mrow> <mo>(</mo> <mn>1</mn> <mo>)</mo> </mrow> </math> is the inversion of <math xmlns="http://www.w3.org/1998/Math/MathML"> <msub> <mi>ℤ</mi> <mi>N</mi> </msub> </math>). It is well-known that there exists a reduction to the case where the hidden subgroup is <math xmlns="http://www.w3.org/1998/Math/MathML"> <mi>H</mi> <mo>=</mo> <mrow> <mo>⟨</mo> <mrow> <mo>(</mo> <mi>d</mi> <mo>,</mo> <mn>1</mn> <mo>)</mo> </mrow> <mo>⟩</mo> </mrow> </math> for some <math xmlns="http://www.w3.org/1998/Math/MathML"> <mrow> <mi>d</mi> <mo>∈</mo> <msub> <mi>ℤ</mi> <mi>N</mi> </msub> </mrow> </math>. In that case, if we fix <math xmlns="http://www.w3.org/1998/Math/MathML"> <mrow> <mi>b</mi> <mo>∈</mo> <mrow> <mo>{</mo> <mn>0</mn> <mo>,</mo> <mn>1</mn> <mo>}</mo> </mrow> </mrow> </math>, the elements <math xmlns="http://www.w3.org/1998/Math/MathML"> <mrow> <mo>(</mo> <mrow> <mi>i</mi> <mo>,</mo> <mi>b</mi> </mrow> <mo>)</mo> </mrow> </math> for <math xmlns="http://www.w3.org/1998/Math/MathML"> <mrow> <mi>i</mi> <mo>∈</mo> <msub> <mi>ℤ</mi> <mi>N</mi> </msub> </mrow> </math> form a complete set of coset representatives, so <math xmlns="http://www.w3.org/1998/Math/MathML"> <mi>f</mi> </math> is one-to-one over <math xmlns="http://www.w3.org/1998/Math/MathML"> <mrow> <msub> <mi>ℤ</mi> <mi>N</mi> </msub> <mo>×</mo> <mrow> <mo>{</mo> <mi>b</mi> <mo>}</mo> </mrow> </mrow> </math>. Thus, <math xmlns="http://www.w3.org/1998/Math/MathML"> <mrow> <mi>x</mi> <mo>↦</mo> <mrow> <mi>f</mi> <mrow> <mo>(</mo> <mrow> <mi>x</mi> <mo>,</mo> <mi>b</mi> </mrow> <mo>)</mo> </mrow> </mrow> </mrow> </math> is a <em>permutation</em> of <math xmlns="http://www.w3.org/1998/Math/MathML"> <msub> <mi>ℤ</mi> <mi>N</mi> </msub> </math>, a property that will be used below to construct a unitary transform.</p>

<p>First let's recall the classical inductive method to determine <math xmlns="http://www.w3.org/1998/Math/MathML"> <mi>d</mi> </math>. If <math xmlns="http://www.w3.org/1998/Math/MathML"> <mi>M</mi> </math> is a divisor of <math xmlns="http://www.w3.org/1998/Math/MathML"> <mi>N</mi> </math>, let <math xmlns="http://www.w3.org/1998/Math/MathML"> <mrow> <mi>N</mi> <mo>'</mo> </mrow> <mo>=</mo> <mfrac> <mi>N</mi> <mi>M</mi> </mfrac> </math> and write the euclidean division <math xmlns="http://www.w3.org/1998/Math/MathML"> <mi>d</mi> <mo>=</mo> <mi>M</mi> <mrow> <mi>d</mi> <mo>'</mo> </mrow> <mo>+</mo> <mi>r</mi> </math>. If we are able to determine <math xmlns="http://www.w3.org/1998/Math/MathML"> <mi>r</mi> </math> in polynomial time, then we can define the oracle <math xmlns="http://www.w3.org/1998/Math/MathML"> <mrow> <mrow> <mi>f</mi> <mo>'</mo> </mrow> <mrow> <mo>(</mo> <mi>x</mi> <mo>,</mo> <mi>y</mi> <mo>)</mo> </mrow> </mrow> <mo>=</mo> <mi>f</mi> <mrow> <mo>(</mo> <mrow> <mi>M</mi> <mi>x</mi> <mo>+</mo> <mi>r</mi> </mrow> <mo>,</mo> <mi>y</mi> <mo>)</mo> </mrow> </math> for <math xmlns="http://www.w3.org/1998/Math/MathML"> <mrow> <mi>x</mi> <mo>∈</mo> <msub> <mi>ℤ</mi> <mrow> <mi>N</mi> <mo>'</mo> </mrow> </msub> </mrow> </math> and <math xmlns="http://www.w3.org/1998/Math/MathML"> <mrow> <mi>y</mi> <mo>∈</mo> <msub> <mi>ℤ</mi> <mn>2</mn> </msub> </mrow> </math> and obtain a dihedral HSP with hidden subgroup <math xmlns="http://www.w3.org/1998/Math/MathML"> <mrow> <mo>⟨</mo> <mrow> <mo>(</mo> <mrow> <mi>d</mi> <mo>'</mo> </mrow> <mo>,</mo> <mn>1</mn> <mo>)</mo> </mrow> <mo>⟩</mo> </mrow> </math>. Since the prime factorization has only <math xmlns="http://www.w3.org/1998/Math/MathML"> <mrow> <mi>O</mi> <mrow> <mo>(</mo> <mrow> <mi>log</mi> <mi>N</mi> </mrow> <mo>)</mo> </mrow> </mrow> </math> factors, we can repeat this inductive step to get an efficient algorithm. Of course, this is likely to be useful only when the factors are small for otherwise it may be as much difficult to determine <math xmlns="http://www.w3.org/1998/Math/MathML"> <mi>r</mi> </math> as to determine the whole <math xmlns="http://www.w3.org/1998/Math/MathML"> <mi>d</mi> </math>. One interesting case is <math xmlns="http://www.w3.org/1998/Math/MathML"> <mi>N</mi> <mo>=</mo> <msup> <mn>2</mn> <mi>n</mi> </msup> </math> and <math xmlns="http://www.w3.org/1998/Math/MathML"> <mi>M</mi> <mo>=</mo> <mn>2</mn> </math>: at each step, <math xmlns="http://www.w3.org/1998/Math/MathML"> <mi>N</mi> </math> remains a power of 2 and we determine the parity of <math xmlns="http://www.w3.org/1998/Math/MathML"> <mi>d</mi> </math>.</p>

<p>For <math xmlns="http://www.w3.org/1998/Math/MathML"> <mn>0</mn> <mo>≤</mo> <mi>l</mi> <mo>&lt;</mo> <mi>M</mi> </math>, we consider the <math xmlns="http://www.w3.org/1998/Math/MathML"> <mi>N</mi> <mo>'</mo> </math>-dimensional subspace spanned by the vectors <math xmlns="http://www.w3.org/1998/Math/MathML"> <mrow> <mo stretchy="false">∣</mo> <mi>l</mi> <mrow> <mi>N</mi> <mo>'</mo> </mrow> <mo>+</mo> <mi>m</mi> <mo stretchy="false">⟩</mo> </mrow> </math> for <math xmlns="http://www.w3.org/1998/Math/MathML"> <mn>0</mn> <mo>≤</mo> <mi>m</mi> <mo>&lt;</mo> <mi>N</mi> <mo>'</mo> </math>. Since these <math xmlns="http://www.w3.org/1998/Math/MathML"> <mi>M</mi> </math> subspaces are orthogonal, we can construct a unitary transform by applying a Quantum Fourier Transform <math xmlns="http://www.w3.org/1998/Math/MathML"> <msub> <mi>F</mi> <mrow> <mi>N</mi> <mo>'</mo> </mrow> </msub> </math> on each subspace separately. Finally, we apply the permutation mentionned at the beginning for <math xmlns="http://www.w3.org/1998/Math/MathML"> <mi>b</mi> <mo>=</mo> <mn>0</mn> </math>. We get a unitary transform <math xmlns="http://www.w3.org/1998/Math/MathML"> <mi>W</mi> </math> below where <math xmlns="http://www.w3.org/1998/Math/MathML"> <mi>x</mi> <mo>=</mo> <mi>M</mi> <mi>i</mi> <mo>+</mo> <mi>k</mi> </math> is the euclidean division of <math xmlns="http://www.w3.org/1998/Math/MathML"> <mi>x</mi> </math> by <math xmlns="http://www.w3.org/1998/Math/MathML"> <mi>M</mi> </math>:</p>

<p><math display="block" xmlns="http://www.w3.org/1998/Math/MathML"> <mo>∀</mo> <mrow> <mi>x</mi> <mo>∈</mo> <msub> <mi>Z</mi> <mi>N</mi> </msub> </mrow> <mo>,</mo> <mrow> <mi>W</mi> <mrow> <mo stretchy="false">∣</mo> <mi>x</mi> <mo stretchy="false">⟩</mo> </mrow> </mrow> <mo>=</mo> <mrow> <mfrac> <mn>1</mn> <msqrt> <mrow> <mi>N</mi> <mo>′</mo> </mrow> </msqrt> </mfrac> <munderover> <mo lspace="thinmathspace" rspace="thinmathspace">∑</mo> <mrow> <mi>j</mi> <mo>=</mo> <mn>0</mn> </mrow> <mrow> <mrow> <mi>N</mi> <mo>′</mo> </mrow> <mo>−</mo> <mn>1</mn> </mrow> </munderover> <mrow> <msup> <mi>ⅇ</mi> <mrow> <mn>2</mn> <mi>ⅈ</mi> <mi>π</mi> <mfrac> <mrow> <mi>i</mi> <mi>j</mi> </mrow> <mrow> <mi>N</mi> <mo>′</mo> </mrow> </mfrac> </mrow> </msup> <mrow> <mo stretchy="false">∣</mo> <mrow> <mi>f</mi> <mo stretchy="false">(</mo> <mrow> <mi>M</mi> <mi>j</mi> <mo>+</mo> <mi>k</mi> </mrow> <mo>,</mo> <mn>0</mn> <mo stretchy="false">)</mo> </mrow> <mo stretchy="false">⟩</mo> </mrow> </mrow> </mrow> </math></p>

<p>Now, let's consider the superposition (again, we see that it is well-defined by considering the permutation mentionned at the beginning for <math xmlns="http://www.w3.org/1998/Math/MathML"> <mi>b</mi> <mo>=</mo> <mn>1</mn> </math>):</p>

<p><math display="block" xmlns="http://www.w3.org/1998/Math/MathML"> <mfrac> <mn>1</mn> <msqrt> <mrow> <mi>N</mi> <mo>′</mo> </mrow> </msqrt> </mfrac> <munderover> <mo lspace="thinmathspace" rspace="thinmathspace">∑</mo> <mrow> <mi>i</mi> <mo>=</mo> <mn>0</mn> </mrow> <mrow> <mrow> <mi>N</mi> <mo>′</mo> </mrow> <mo>−</mo> <mn>1</mn> </mrow> </munderover> <mrow> <mo stretchy="false">∣</mo> <mrow> <mi>f</mi> <mo stretchy="false">(</mo> <mrow> <mi>M</mi> <mi>i</mi> </mrow> <mo>,</mo> <mn>1</mn> <mo stretchy="false">)</mo> </mrow> <mo stretchy="false">⟩</mo> </mrow> </math></p>

<p>The state can be rewritten, using the fact that <math xmlns="http://www.w3.org/1998/Math/MathML"> <mi>f</mi> </math> is constant on <math xmlns="http://www.w3.org/1998/Math/MathML"> <mi>H</mi> <mo>=</mo> <mrow> <mo>⟨</mo> <mrow> <mo>(</mo> <mi>d</mi> <mo>,</mo> <mn>1</mn> <mo>)</mo> </mrow> <mo>⟩</mo> </mrow> </math>:</p>

<p><math display="block" xmlns="http://www.w3.org/1998/Math/MathML"> <mrow> <mtable columnalign="right left right left right left right left right left" columnspacing="0em"> <mtr> <mtd> <mfrac> <mn>1</mn> <msqrt> <mrow> <mi>N</mi> <mo>′</mo> </mrow> </msqrt> </mfrac> <mrow> <munderover> <mo lspace="thinmathspace" rspace="thinmathspace">∑</mo> <mrow> <mi>i</mi> <mo>=</mo> <mn>0</mn> </mrow> <mrow> <mrow> <mi>N</mi> <mo>′</mo> </mrow> <mo>−</mo> <mn>1</mn> </mrow> </munderover> <mrow> <mo stretchy="false">∣</mo> <mrow> <mi>f</mi> <mo stretchy="false">(</mo> <mrow> <mi>M</mi> <mi>i</mi> </mrow> <mo>,</mo> <mn>1</mn> <mo stretchy="false">)</mo> </mrow> <mo stretchy="false">⟩</mo> </mrow> </mrow> </mtd> <mtd> <mo>=</mo> <mfrac> <mn>1</mn> <msqrt> <mrow> <mi>N</mi> <mo>′</mo> </mrow> </msqrt> </mfrac> <mrow> <munderover> <mo lspace="thinmathspace" rspace="thinmathspace">∑</mo> <mrow> <mi>i</mi> <mo>=</mo> <mn>0</mn> </mrow> <mrow> <mrow> <mi>N</mi> <mo>′</mo> </mrow> <mo>−</mo> <mn>1</mn> </mrow> </munderover> <mrow> <mo stretchy="false">∣</mo> <mrow> <mi>f</mi> <mrow> <mo stretchy="false">(</mo> <mrow> <mrow> <mi>M</mi> <mi>i</mi> </mrow> <mo>−</mo> <mi>d</mi> <mo>,</mo> <mn>0</mn> <mo stretchy="false">)</mo> </mrow> <mrow> <mo stretchy="false">(</mo> <mi>d</mi> <mo>,</mo> <mn>1</mn> <mo stretchy="false">)</mo> </mrow> </mrow> </mrow> <mo stretchy="false">⟩</mo> </mrow> </mrow> </mtd> </mtr> <mtr> <mtd> </mtd> <mtd> <mo>=</mo> <mfrac> <mn>1</mn> <msqrt> <mrow> <mi>N</mi> <mo>′</mo> </mrow> </msqrt> </mfrac> <mrow> <munderover> <mo lspace="thinmathspace" rspace="thinmathspace">∑</mo> <mrow> <mi>i</mi> <mo>=</mo> <mn>0</mn> </mrow> <mrow> <mrow> <mi>N</mi> <mo>′</mo> </mrow> <mo>−</mo> <mn>1</mn> </mrow> </munderover> <mrow> <mo stretchy="false">∣</mo> <mrow> <mi>f</mi> <mrow> <mo stretchy="false">(</mo> <mrow> <mrow> <mi>M</mi> <mi>i</mi> </mrow> <mo>−</mo> <mi>d</mi> <mo>,</mo> <mn>0</mn> <mo stretchy="false">)</mo> </mrow> </mrow> </mrow> <mo stretchy="false">⟩</mo> </mrow> </mrow> </mtd> </mtr> <mtr> <mtd> </mtd> <mtd> <mo>=</mo> <mfrac> <mn>1</mn> <msqrt> <mrow> <mi>N</mi> <mo>′</mo> </mrow> </msqrt> </mfrac> <mrow> <munderover> <mo lspace="thinmathspace" rspace="thinmathspace">∑</mo> <mrow> <mi>i</mi> <mo>=</mo> <mn>0</mn> </mrow> <mrow> <mrow> <mi>N</mi> <mo>′</mo> </mrow> <mo>−</mo> <mn>1</mn> </mrow> </munderover> <mrow> <mo stretchy="false">∣</mo> <mrow> <mi>f</mi> <mrow> <mo stretchy="false">(</mo> <mrow> <mrow> <mi>M</mi> <mi>i</mi> </mrow> <mo>−</mo> <mrow> <mo>(</mo> <mrow> <mi>M</mi> <mrow> <mi>d</mi> <mo>′</mo> </mrow> <mo>+</mo> <mi>r</mi> </mrow> <mo>)</mo> </mrow> </mrow> <mo>,</mo> <mn>0</mn> <mo stretchy="false">)</mo> </mrow> </mrow> <mo stretchy="false">⟩</mo> </mrow> </mrow> </mtd> </mtr> <mtr> <mtd> </mtd> <mtd> <mo>=</mo> <mfrac> <mn>1</mn> <msqrt> <mrow> <mi>N</mi> <mo>′</mo> </mrow> </msqrt> </mfrac> <mrow> <munderover> <mo lspace="thinmathspace" rspace="thinmathspace">∑</mo> <mrow> <mi>i</mi> <mo>=</mo> <mn>0</mn> </mrow> <mrow> <mrow> <mi>N</mi> <mo>′</mo> </mrow> <mo>−</mo> <mn>1</mn> </mrow> </munderover> <mrow> <mo stretchy="false">∣</mo> <mrow> <mi>f</mi> <mo stretchy="false">(</mo> <mrow> <mrow> <mi>M</mi> <mrow> <mo stretchy="false">(</mo> <mi>i</mi> <mo>−</mo> <mrow> <mi>d</mi> <mo>′</mo> </mrow> <mo>+</mo> <mrow> <mo stretchy="false">(</mo> <mi>N</mi> <mo>′</mo> <mo lspace="verythinmathspace" rspace="0em">−</mo> <mn>1</mn> <mo stretchy="false">)</mo> </mrow> <mo stretchy="false">)</mo> </mrow> </mrow> <mo>+</mo> <mrow> <mo stretchy="false">(</mo> <mi>M</mi> <mo>−</mo> <mi>r</mi> <mo stretchy="false">)</mo> </mrow> </mrow> <mo>,</mo> <mn>0</mn> <mo stretchy="false">)</mo> </mrow> <mo stretchy="false">⟩</mo> </mrow> </mrow> </mtd> </mtr> <mtr> <mtd> </mtd> <mtd> <mo>=</mo> <mfrac> <mn>1</mn> <msqrt> <mrow> <mi>N</mi> <mo>′</mo> </mrow> </msqrt> </mfrac> <mrow> <munderover> <mo lspace="thinmathspace" rspace="thinmathspace">∑</mo> <mrow> <mi>i</mi> <mo>=</mo> <mn>0</mn> </mrow> <mrow> <mrow> <mi>N</mi> <mo>′</mo> </mrow> <mo>−</mo> <mn>1</mn> </mrow> </munderover> <mrow> <mo stretchy="false">∣</mo> <mrow> <mi>f</mi> <mo stretchy="false">(</mo> <mrow> <mrow> <mi>M</mi> <mi>i</mi> </mrow> <mo>+</mo> <mrow> <mo stretchy="false">(</mo> <mi>M</mi> <mo>−</mo> <mi>r</mi> <mo stretchy="false">)</mo> </mrow> </mrow> <mo>,</mo> <mn>0</mn> <mo stretchy="false">)</mo> </mrow> <mo stretchy="false">⟩</mo> </mrow> </mrow> </mtd> </mtr> </mtable> </mrow> </math></p>

<p> </p>

<p>Applying <math xmlns="http://www.w3.org/1998/Math/MathML"> <msup> <mi>W</mi> <mrow> <mo>−</mo> <mn>1</mn> </mrow> </msup> </math> to this state gives <math xmlns="http://www.w3.org/1998/Math/MathML"> <mrow> <mo stretchy="false">∣</mo> <mrow> <mi>M</mi> <mo>−</mo> <mi>r</mi> </mrow> <mo>&nbsp;</mo> <mi>mod</mi> <mo>&nbsp;</mo> <mrow> <mo>(</mo> <mi>M</mi> <mo>)</mo> </mrow> <mo stretchy="false">⟩</mo> </mrow> </math> and so the value of <math xmlns="http://www.w3.org/1998/Math/MathML"> <mi>r</mi> </math> by a measurement in the standard basis.</p>

<p>Two questions remain: can we implement <math xmlns="http://www.w3.org/1998/Math/MathML"> <mi>W</mi> </math> and create the state <math xmlns="http://www.w3.org/1998/Math/MathML"> <mrow> <mo stretchy="false">∣</mo> <mi>Ψ</mi> <mo stretchy="false">⟩</mo> </mrow> </math> efficiently? If <math xmlns="http://www.w3.org/1998/Math/MathML"> <mi>N</mi> <mo>=</mo> <msup> <mn>2</mn> <mi>n</mi> </msup> </math> and <math xmlns="http://www.w3.org/1998/Math/MathML"> <mi>M</mi> <mo>=</mo> <mn>2</mn> </math>, there are many simplifications because we are working with qubits. In that case, it is easy to see that the answer to the previous questions is affirmative if we have gates <math xmlns="http://www.w3.org/1998/Math/MathML"> <msub> <mi>V</mi> <mrow> <mi>f</mi> <mo>,</mo> <mi>b</mi> </mrow> </msub> <mrow> <mo stretchy="false">∣</mo> <mi>x</mi> <mo stretchy="false">⟩</mo> </mrow> <mo>=</mo> <mrow> <mo>∣</mo> <mrow> <mi>f</mi> <mrow> <mo>(</mo> <mrow> <mi>x</mi> <mo>,</mo> <mi>b</mi> </mrow> <mo>)</mo> </mrow> <mo stretchy="false">⟩</mo> </mrow> </mrow> </math> implementing the permutation mentioned at the beginning. However, it is not clear how to build <math xmlns="http://www.w3.org/1998/Math/MathML"> <msub> <mi>V</mi> <mrow> <mi>f</mi> <mo>,</mo> <mi>b</mi> </mrow> </msub> </math> from the gate <math xmlns="http://www.w3.org/1998/Math/MathML"> <msub> <mi>U</mi> <mi>f</mi> </msub> </math> generally given in the classical presentation of the problem...</p>

<p>update: OK, there is also the trivial solution <math xmlns="http://www.w3.org/1998/Math/MathML"> <mi>N</mi> <mo>=</mo> <mi>M</mi> <mo>,</mo> <mrow> <mi>N</mi> <mo>'</mo> </mrow> <mo>=</mo> <mn>1</mn> </math>where the algorithm above is just computing <math xmlns="http://www.w3.org/1998/Math/MathML"> <mrow> <msubsup> <mi>V</mi> <mrow> <mi>f</mi> <mo>,</mo> <mn>0</mn> </mrow> <mrow> <mo>−</mo> <mn>1</mn> </mrow> </msubsup> <msub> <mi>V</mi> <mrow> <mi>f</mi> <mo>,</mo> <mn>1</mn> </mrow> </msub> <mrow> <mo stretchy="false">∣</mo> <mn>0</mn> <mo stretchy="false">⟩</mo> </mrow> </mrow> <mo>=</mo> <mrow> <mo stretchy="false">∣</mo> <mrow> <mi>N</mi> <mo>−</mo> <mi>d</mi> </mrow> <mo>&nbsp;</mo> <mi>mod</mi> <mo>&nbsp;</mo> <mrow> <mo>(</mo> <mi>N</mi> <mo>)</mo> </mrow> <mo stretchy="false">⟩</mo> </mrow> </math>. However, I'm still wondering if there is a way to modify the previous method to work with <math xmlns="http://www.w3.org/1998/Math/MathML"> <msub> <mi>U</mi> <mi>f</mi> </msub> </math>.</p>

{% endraw %}
